Foundation/Modal/Kripke/Logic/K.lean
@@ -8,19 +8,19 @@ namespace LO.Modal
 open Kripke
 open Hilbert.Kripke
 
-namespace Hilbert.K.Kripke
+namespace Logic.K.Kripke
 
-instance sound : Sound (Hilbert.K) FrameClass.all := instSound_of_validates_axioms FrameClass.all.validates_axiomK
+instance sound : Sound (Logic.K) FrameClass.all := instSound_of_validates_axioms FrameClass.all.validates_axiomK
 
-instance sound_finite : Sound (Hilbert.K) FrameClass.finite_all := instSound_of_validates_axioms FrameClass.finite_all.validates_axiomK
+instance sound_finite : Sound (Logic.K) FrameClass.finite_all := instSound_of_validates_axioms FrameClass.finite_all.validates_axiomK
 
-instance : Entailment.Consistent (Hilbert.K) := consistent_of_sound_frameclass FrameClass.all (by simp)
+instance : Entailment.Consistent (Logic.K) := consistent_of_sound_frameclass FrameClass.all (by simp)
 
-instance : Kripke.Canonical (Hilbert.K) FrameClass.all := ⟨by trivial⟩
+instance : Kripke.Canonical (Logic.K) FrameClass.all := ⟨by trivial⟩
 
-instance complete : Complete (Hilbert.K) FrameClass.all := inferInstance
+instance complete : Complete (Logic.K) FrameClass.all := inferInstance
 
-instance complete_finite : Complete (Hilbert.K) (FrameClass.finite_all) := ⟨by
+instance complete_finite : Complete (Logic.K) (FrameClass.finite_all) := ⟨by
   intro φ hp;
   apply Kripke.complete.complete;
   intro F _ V x;
@@ -33,21 +33,10 @@ instance complete_finite : Complete (Hilbert.K) (FrameClass.finite_all) := ⟨by
   simp;
 ⟩
 
-end Hilbert.K.Kripke
+lemma all : Logic.K = FrameClass.all.logic := eq_hilbert_logic_frameClass_logic
+lemma finite_all : Logic.K = FrameClass.finite_all.logic := eq_hilbert_logic_frameClass_logic
 
+end Logic.K.Kripke
 
-namespace Logic
-
-lemma K.Kripke.all : Logic.K = FrameClass.all.logic := eq_hilbert_logic_frameClass_logic
-lemma K.Kripke.finite_all : Logic.K = FrameClass.finite_all.logic := eq_hilbert_logic_frameClass_logic
-
-theorem K.proper_extension_of_Empty : Logic.Empty ⊂ Logic.K := by
-  constructor;
-  . simp;
-  . suffices ∃ φ, Hilbert.K ⊢! φ by tauto_set;
-    use ⊤;
-    simp;
-
-end Logic
 
 end LO.Modal
