Foundation/Modal/Logic/Basic.lean
@@ -1,27 +1,113 @@
 import Foundation.Modal.Formula
+import Foundation.Modal.Entailment.Basic
 
 namespace LO.Modal
 
-abbrev Logic := Set (Modal.Formula ℕ)
+open LO.Entailment
+open Entailment
+
+variable {α : Type*}
+
+abbrev Logic (α) := Set (Modal.Formula α)
+
+instance : Entailment (Formula α) (Logic α) := ⟨fun L φ ↦ PLift (φ ∈ L)⟩
+
 
 namespace Logic
 
-class Consistent (L : Logic) : Prop where
-  consis : L ≠ Set.univ
-attribute [simp] Consistent.consis
+variable {L L₀ L₁ L₂ L₃ : Logic α}
+
+section
+
+protected class Substitution (L : Logic α) where
+  subst {φ} (s) : L ⊢ φ → L ⊢ φ⟦s⟧
+
+protected class IsQuasiNormal (L : Logic α) extends Entailment.Cl L, Entailment.HasAxiomK L, Entailment.HasDiaDuality L, L.Substitution where
+
+protected class IsNormal (L : Logic α) extends L.IsQuasiNormal, Entailment.Necessitation L where
+instance [L.IsNormal] : Entailment.K L where
+
+end
 
 
-protected class Unnecessitation (L : Logic) where
-  unnec_closed {φ} : □φ ∈ L → φ ∈ L
+section
 
-protected class ModalDisjunctive (L : Logic) where
-  modal_disjunctive_closed {φ ψ} : □φ ⋎ □ψ ∈ L → φ ∈ L ∨ ψ ∈ L
+variable {L : Logic α} {φ ψ : Formula α}
+
+@[simp low]
+lemma iff_provable : L ⊢! φ ↔ φ ∈ L := by
+  constructor;
+  . intro h;
+    exact PLift.down h.some;
+  . intro h;
+    constructor;
+    constructor;
+    exact h;
+
+@[simp low]
+lemma iff_unprovable : L ⊬ φ ↔ φ ∉ L := by
+  apply not_congr;
+  simp [iff_provable];
+
+lemma iff_equal_provable_equiv : L₁ = L₂ ↔ L₁ ≊ L₂ := by
+  constructor;
+  . tauto;
+  . rintro h;
+    ext φ;
+    simpa using Equiv.iff.mp h φ;
+
+lemma subst! [L.Substitution] (s : Substitution _) (hφ : L ⊢! φ) : L ⊢! φ⟦s⟧ := ⟨Substitution.subst s hφ.some⟩
+
+
+section
+
+variable [DecidableEq α] [L.IsQuasiNormal] [Consistent L]
+
+@[simp]
+lemma no_bot : L ⊬ ⊥ := by
+  obtain ⟨φ, hφ⟩ := Consistent.exists_unprovable (𝓢 := L) inferInstance;
+  by_contra! hC;
+  apply hφ;
+  apply of_O!;
+  exact hC;
+
+-- TODO: more general place
+lemma not_neg_of! (hφ : L ⊢! φ) : L ⊬ ∼φ := by
+  by_contra! hC;
+  apply L.no_bot;
+  exact hC ⨀ hφ;
+
+end
+
+end
 
 end Logic
 
 
-protected abbrev Logic.Empty : Logic := ∅
+section
 
-protected abbrev Logic.Univ : Logic := Set.univ
+variable {L : Logic α}
+
+instance : (∅ : Logic α) ⪯ L := ⟨by simp [Entailment.theory]⟩
+
+instance [HasAxiomVerum L] : (∅ : Logic α) ⪱ L := by
+  apply strictlyWeakerThan_iff.mpr;
+  constructor;
+  . simp;
+  . use ⊤; constructor <;> simp;
+
+instance : L ⪯ (Set.univ : Logic α) := ⟨by simp [Entailment.theory]⟩
+
+instance [Consistent L] : L ⪱ (Set.univ : Logic α) := by
+  apply strictlyWeakerThan_iff.mpr;
+  constructor;
+  . simp;
+  . obtain ⟨φ, hφ⟩ := consistent_iff_exists_unprovable (𝓢 := L) |>.mp (by assumption);
+    use φ;
+    constructor;
+    . assumption;
+    . simp [Entailment.theory]
+
+end
 
 end LO.Modal
