Foundation/Modal/ModalCompanion/Basic.lean
@@ -15,22 +15,46 @@ def Propositional.Formula.goedelTranslate : Propositional.Formula α → Modal.F
   | φ ➝ ψ => □((goedelTranslate φ) ➝ (goedelTranslate ψ))
 postfix:90 "ᵍ" => Propositional.Formula.goedelTranslate
 
-class Modal.ModalCompanion (IL : Propositional.Logic) (ML : Modal.Logic) where
-  companion : ∀ {φ}, φ ∈ IL ↔ φᵍ ∈ ML
+class Modal.ModalCompanion (IL : Propositional.Logic) (ML : Modal.Logic _) where
+  companion : ∀ {φ}, φ ∈ IL ↔ ML ⊢! φᵍ
 
-lemma Modal.instModalCompanion (h₁ : ∀ {φ}, φ ∈ IL → φᵍ ∈ ML) (h₂ : ∀ {φ}, φᵍ ∈ ML → φ ∈ IL) : Modal.ModalCompanion IL ML := ⟨λ {_} => ⟨h₁, h₂⟩⟩
+lemma Modal.instModalCompanion (h₁ : ∀ {φ}, φ ∈ IL → ML ⊢! φᵍ) (h₂ : ∀ {φ}, ML ⊢! φᵍ → φ ∈ IL) : Modal.ModalCompanion IL ML := ⟨λ {_} => ⟨h₁, h₂⟩⟩
 
 
 namespace Propositional.Logic
 
 variable {IL : Propositional.Logic}
 
-def smallestMC (IL : Propositional.Logic) : Modal.Logic := Modal.Logic.sumNormal Modal.Logic.S4 { φᵍ | φ ∈ IL }
+abbrev smallestMC (IL : Propositional.Logic) : Modal.Logic ℕ := Modal.Logic.sumNormal Modal.Logic.S4 { φᵍ | φ ∈ IL }
 
-lemma smallestMC.mdp_S4 (hφψ : Modal.Hilbert.S4 ⊢! φ ➝ ψ) (hφ : φ ∈ IL.smallestMC)
-  : ψ ∈ IL.smallestMC := Modal.Logic.sumNormal.mdp (Modal.Logic.sumNormal.mem₁ hφψ) hφ
+instance : Modal.Entailment.S4 IL.smallestMC where
+  T φ := by
+    constructor;
+    apply Modal.Logic.iff_provable.mp;
+    apply Modal.Logic.subst! (φ := Modal.Axioms.T (.atom 0)) (s := λ _ => φ);
+    apply Modal.Logic.sumNormal.mem₁!;
+    simp;
+  Four φ := by
+    constructor;
+    apply Modal.Logic.iff_provable.mp;
+    apply Modal.Logic.subst! (φ := Modal.Axioms.Four (.atom 0)) (s := λ _ => φ);
+    apply Modal.Logic.sumNormal.mem₁!;
+    simp;
 
-def largestMC (IL : Propositional.Logic) : Modal.Logic := Modal.Logic.addNormal IL.smallestMC (Modal.Axioms.Grz (.atom 0))
+lemma smallestMC.mdp_S4 (hφψ : Modal.Logic.S4 ⊢! φ ➝ ψ) (hφ : IL.smallestMC ⊢! φ) : IL.smallestMC ⊢! ψ := by
+  exact (Modal.Logic.sumNormal.mem₁! hφψ) ⨀ hφ;
+
+abbrev largestMC (IL : Propositional.Logic) : Modal.Logic ℕ := Modal.Logic.sumNormal IL.smallestMC { Modal.Axioms.Grz (.atom 0) }
+
+instance : Modal.Entailment.Grz IL.largestMC where
+  Grz φ := by
+    constructor;
+    apply Modal.Logic.iff_provable.mp;
+    apply Modal.Logic.subst! (φ := Modal.Axioms.Grz (.atom 0)) (s := λ _ => φ);
+    apply Modal.Logic.sumNormal.mem₂!;
+    simp;
+
+instance : IL.smallestMC ⪯ IL.smallestMC := inferInstance
 
 end Propositional.Logic
 
@@ -42,12 +66,12 @@ open Propositional.Formula (goedelTranslate)
 lemma Modal.instModalCompanion_of_smallestMC_via_KripkeSemantics
   {IL : Propositional.Logic}
   (IC : Propositional.Kripke.FrameClass) (hIL_complete : ∀ {φ}, φ ∈ IL ↔ φ ∈ IC.logic)
-  (MC : Modal.Kripke.FrameClass) (hML_complete : ∀ {φ}, φ ∈ IL.smallestMC ↔ φ ∈ MC.logic)
+  (MC : Modal.Kripke.FrameClass) (hML_complete : ∀ {φ}, IL.smallestMC ⊢! φ ↔ MC.logic ⊢! φ)
   (hIC_MC : ∀ F ∈ IC, ⟨F.World, F.Rel⟩ ∈ MC)
   : ModalCompanion IL (IL.smallestMC) := Modal.instModalCompanion
   (by
     intro φ hφ;
-    apply Modal.Logic.sumNormal.mem₂;
+    apply Modal.Logic.sumNormal.mem₂!;
     use φ;
   )
   (by
@@ -81,6 +105,7 @@ lemma Modal.instModalCompanion_of_smallestMC_via_KripkeSemantics
           . right; exact ihq x |>.mpr hq;
       | _ => simp_all [goedelTranslate, Propositional.Formula.Kripke.Satisfies, Modal.Formula.Kripke.Satisfies];
     apply hML_complete.not.mpr;
+    simp only [Logic.iff_provable, Set.mem_setOf_eq];
     apply Modal.Kripke.not_validOnFrameClass_of_exists_frame;
     use { World := F.World, Rel := F.Rel };
     constructor;
@@ -94,13 +119,13 @@ lemma Modal.instModalCompanion_of_smallestMC_via_KripkeSemantics
 lemma Modal.instModalCompanion_of_largestMC_via_KripkeSemantics
   {IL : Propositional.Logic}
   (IC : Propositional.Kripke.FrameClass) (hIL_complete : ∀ {φ}, φ ∈ IL ↔ φ ∈ IC.logic)
-  (MC : Modal.Kripke.FrameClass) (hML_complete : ∀ {φ}, φ ∈ IL.largestMC ↔ φ ∈ MC.logic)
+  (MC : Modal.Kripke.FrameClass) (hML_complete : ∀ {φ}, IL.largestMC ⊢! φ ↔ MC.logic ⊢! φ)
   (hIC_MC : ∀ F ∈ IC, ⟨F.World, F.Rel⟩ ∈ MC)
   : ModalCompanion IL (IL.largestMC) := Modal.instModalCompanion
   (by
     intro φ hφ;
-    apply Modal.Logic.sumNormal.mem₁;
-    apply Modal.Logic.sumNormal.mem₂;
+    apply Modal.Logic.sumNormal.mem₁!;
+    apply Modal.Logic.sumNormal.mem₂!;
     use φ;
   )
   (by
@@ -136,6 +161,7 @@ lemma Modal.instModalCompanion_of_largestMC_via_KripkeSemantics
           . right; exact ihq x |>.mpr hq;
       | _ => simp_all [goedelTranslate, Propositional.Formula.Kripke.Satisfies, Modal.Formula.Kripke.Satisfies];
     apply hML_complete.not.mpr;
+    simp only [Logic.iff_provable, Set.mem_setOf_eq];
     apply Modal.Kripke.not_validOnFrameClass_of_exists_frame;
     use { World := F.World, Rel := F.Rel };
     constructor;
@@ -149,46 +175,46 @@ lemma Modal.instModalCompanion_of_largestMC_via_KripkeSemantics
 end
 
 
-namespace Modal.Hilbert
+namespace Modal
 
 open Propositional.Formula (goedelTranslate)
 
-variable {IL : Propositional.Logic} {ML : Modal.Logic}
-variable {IH : Propositional.Hilbert ℕ} {MH : Modal.Hilbert ℕ}
+variable {IL : Propositional.Logic} {ML : Modal.Logic ℕ}
+variable {IH : Propositional.Hilbert ℕ}
 variable {φ ψ χ : Propositional.Formula ℕ}
 
-variable [Entailment.S4 MH]
+variable [Entailment.S4 ML]
 
-lemma goedelTranslated_axiomTc : MH ⊢! φᵍ ➝ □φᵍ := by
+lemma goedelTranslated_axiomTc : ML ⊢! φᵍ ➝ □φᵍ := by
   induction φ using Propositional.Formula.rec' with
   | hfalsum => simp only [goedelTranslate, efq!];
   | hand φ ψ ihp ihq => exact C!_trans (CKK!_of_C!_of_C! ihp ihq) collect_box_and!
   | hor φ ψ ihp ihq => exact C!_trans (left_A!_intro (right_A!_intro_left ihp) (right_A!_intro_right ihq)) collect_box_or!
   | _ => simp only [goedelTranslate, axiomFour!];
 
-lemma goedelTranslated_implyS : MH ⊢! (φ ➝ ψ ➝ φ)ᵍ := by
+lemma goedelTranslated_implyS : ML ⊢! (φ ➝ ψ ➝ φ)ᵍ := by
   exact nec! $ C!_trans goedelTranslated_axiomTc $ axiomK'! $ nec! $ imply₁!;
 
-lemma goedelTranslated_implyK : MH ⊢! ((φ ➝ ψ ➝ χ) ➝ (φ ➝ ψ) ➝ φ ➝ χ)ᵍ := by
+lemma goedelTranslated_implyK : ML ⊢! ((φ ➝ ψ ➝ χ) ➝ (φ ➝ ψ) ➝ φ ➝ χ)ᵍ := by
   apply nec! $ C!_trans (C!_trans (axiomK'! $ nec! ?b) axiomFour!) $ axiomK'! $ nec! $ C!_trans (axiomK'! $ nec! imply₂!) axiomK!;
   apply provable_iff_provable.mpr;
   apply deduct_iff.mpr;
   apply deduct_iff.mpr;
-  have : [φᵍ, φᵍ ➝ □(ψᵍ ➝ χᵍ)] ⊢[MH]! φᵍ := by_axm!;
-  have : [φᵍ, φᵍ ➝ □(ψᵍ ➝ χᵍ)] ⊢[MH]! (φᵍ ➝ □(ψᵍ ➝ χᵍ)) := by_axm!;
-  have : [φᵍ, φᵍ ➝ □(ψᵍ ➝ χᵍ)] ⊢[MH]! □(ψᵍ ➝ χᵍ) := (by assumption) ⨀ (by assumption);
+  have : [φᵍ, φᵍ ➝ □(ψᵍ ➝ χᵍ)] ⊢[ML]! φᵍ := by_axm!;
+  have : [φᵍ, φᵍ ➝ □(ψᵍ ➝ χᵍ)] ⊢[ML]! (φᵍ ➝ □(ψᵍ ➝ χᵍ)) := by_axm!;
+  have : [φᵍ, φᵍ ➝ □(ψᵍ ➝ χᵍ)] ⊢[ML]! □(ψᵍ ➝ χᵍ) := (by assumption) ⨀ (by assumption);
   exact axiomT'! this;
 
-lemma goedelTranslated_AndIntro : MH ⊢! (φ ➝ ψ ➝ φ ⋏ ψ)ᵍ := by
+lemma goedelTranslated_AndIntro : ML ⊢! (φ ➝ ψ ➝ φ ⋏ ψ)ᵍ := by
   exact nec! $ C!_trans goedelTranslated_axiomTc $ axiomK'! $ nec! $ and₃!
 
-lemma goedelTranslated_OrElim : MH ⊢! (((φ ➝ χ) ➝ (ψ ➝ χ) ➝ (φ ⋎ ψ ➝ χ)))ᵍ := by
+lemma goedelTranslated_OrElim : ML ⊢! (((φ ➝ χ) ➝ (ψ ➝ χ) ➝ (φ ⋎ ψ ➝ χ)))ᵍ := by
   exact nec! $ C!_trans axiomFour! $ axiomK'! $ nec! $ C!_trans (axiomK'! $ nec! $ or₃!) axiomK!;
 
 lemma provable_goedelTranslated_of_provable
-  (IH : Propositional.Hilbert ℕ) (MH : Modal.Hilbert ℕ) [Entailment.S4 MH]
-  (hAx : ∀ φ ∈ IH.axiomInstances, MH ⊢! φᵍ)
-  : IH ⊢! φ → MH ⊢! φᵍ := by
+  (IH : Propositional.Hilbert ℕ) (ML : Modal.Logic ℕ) [Entailment.S4 ML]
+  (hAx : ∀ φ ∈ IH.axiomInstances, ML ⊢! φᵍ)
+  : IH ⊢! φ → ML ⊢! φᵍ := by
   intro h;
   induction h using Propositional.Hilbert.Deduction.rec! with
   | maxm ih => apply hAx; assumption;
@@ -204,7 +230,7 @@ lemma provable_goedelTranslated_of_provable
   | implyS => exact goedelTranslated_implyS;
   | implyK => exact goedelTranslated_implyK;
 
-end Modal.Hilbert
+end Modal
 
 /-
 lemma dp_of_mdp [ModalDisjunctive mH] [ModalCompanion iH mH] [Entailment.S4 mH] : iH ⊢! φ ⋎ ψ → iH ⊢! φ ∨ iH ⊢! ψ := by
