Foundation/Logic/Entailment.lean
@@ -129,6 +129,8 @@ lemma swk_of_wk_of_swk : 𝓢 ⪯ 𝓣 → 𝓣 ⪱ 𝓤 → 𝓢 ⪱ 𝓤 := by
   · intro h
     exact nh₂ (WeakerThan.trans h h₁)
 
+instance [𝓢 ⪱ 𝓣] : 𝓢 ⪯ 𝓣 := StrictlyWeakerThan.weakerThan
+
 lemma StrictlyWeakerThan.trans : 𝓢 ⪱ 𝓣 → 𝓣 ⪱ 𝓤 → 𝓢 ⪱ 𝓤 := fun h₁ h₂ ↦ swk_of_swk_of_wk h₁ h₂.weakerThan
 
 instance : Trans (α := S) (β := T) (γ := U) (· ⪱ ·) (· ⪯ ·) (· ⪱ ·) where
