Foundation/Modal/Kripke/Hilbert.lean
@@ -7,29 +7,24 @@ open Formula
 open Kripke
 open Formula.Kripke
 
+variable {H : Hilbert ℕ} {Γ : Set (Formula ℕ)} {φ : Formula ℕ}
+variable {F : Kripke.Frame} {C : Kripke.FrameClass}
 
-lemma Logic.eq_hilbert_logic_frameClass_logic
-  {H : Hilbert ℕ} {C : FrameClass} [sound : Sound H C] [complete : Complete H C]
-  : H.logic = C.logic := by
+
+lemma Logic.eq_hilbert_logic_frameClass_logic {H : Hilbert ℕ} {C : FrameClass} [sound : Sound H.logic C] [complete : Complete H.logic C] : H.logic = C.logic := by
   ext φ;
   constructor;
-  . exact sound.sound;
-  . exact complete.complete;
-
+  . intro h;
+    apply sound.sound;
+    simpa;
+  . intro h;
+    simpa using complete.complete h;
 
 namespace Hilbert.Kripke
 
-variable {H : Hilbert ℕ} {Γ : Set (Formula ℕ)} {φ : Formula ℕ}
-
-
-section
-
-variable {C : Kripke.FrameClass}
-
-lemma soundness_of_validates_axiomInstances (hV : C.Validates H.axiomInstances)
-  : H ⊢! φ → C ⊧ φ := by
+lemma soundness_of_validates_axiomInstances (hV : C.Validates H.axiomInstances) : H.logic ⊢! φ → C ⊧ φ := by
   intro hφ F hF;
-  induction hφ using Hilbert.Deduction.rec! with
+  induction hφ with
   | maxm h =>
     obtain ⟨ψ, h, ⟨s, rfl⟩⟩ := h;
     apply hV F hF (ψ⟦s⟧);
@@ -47,13 +42,12 @@ lemma validates_axioms_of_validates_axiomInstances (hV : C.Validates H.axioms) :
   rintro F hF _ ⟨φ, hφ, ⟨s, rfl⟩⟩;
   exact ValidOnFrame.subst $ hV F hF φ hφ;
 
-instance instSound_of_validates_axioms (hV : C.Validates H.axioms) : Sound H C := ⟨fun {_} =>
+instance instSound_of_validates_axioms (hV : C.Validates H.axioms) : Sound H.logic C := ⟨fun {_} =>
   soundness_of_validates_axiomInstances (validates_axioms_of_validates_axiomInstances hV)
 ⟩
 
-lemma consistent_of_sound_frameclass
-  (C : Kripke.FrameClass) (C_nonempty: C.Nonempty := by simp) [sound : Sound H C]
-  : Entailment.Consistent H := by
+lemma consistent_of_sound_frameclass (C : Kripke.FrameClass) (C_nonempty: C.Nonempty := by simp)
+  [sound : Sound H.logic C] : Entailment.Consistent H.logic := by
   apply Entailment.Consistent.of_unprovable (f := ⊥);
   apply not_imp_not.mpr sound.sound;
   apply Semantics.set_models_iff.not.mpr;
@@ -64,17 +58,10 @@ lemma consistent_of_sound_frameclass
   . assumption;
   . simp;
 
-end
 
-
-section
-
-variable {F : Kripke.Frame}
-
-lemma soundness_of_frame_validates_axiomInstances (hV : F ⊧* H.axiomInstances)
-  : H ⊢! φ → F ⊧ φ := by
+lemma soundness_of_frame_validates_axiomInstances (hV : F ⊧* H.axiomInstances) : H.logic ⊢! φ → F ⊧ φ := by
   intro hφ;
-  induction hφ using Hilbert.Deduction.rec! with
+  induction hφ with
   | maxm h =>
     simp only [Semantics.RealizeSet.setOf_iff, ValidOnFrame.models_iff, forall_exists_index, and_imp] at hV;
     obtain ⟨ψ, h, ⟨s, rfl⟩⟩ := h;
@@ -91,19 +78,14 @@ lemma validates_axioms_of_frame_validates_axiomInstances (hV : F ⊧* H.axioms) 
   apply ValidOnFrame.subst;
   exact hV.realize _ hψ;
 
-instance instSound_of_frame_validates_axioms (hV : F ⊧* H.axioms) : Sound H F := ⟨fun {_} =>
+instance instSound_of_frame_validates_axioms (hV : F ⊧* H.axioms) : Sound H.logic F := ⟨fun {_} =>
   soundness_of_frame_validates_axiomInstances (validates_axioms_of_frame_validates_axiomInstances hV)
 ⟩
 
-lemma consistent_of_sound_frames
-  (F : Kripke.Frame) [sound : Sound H F]
-  : Entailment.Consistent H := by
+lemma consistent_of_sound_frames (F : Kripke.Frame) [sound : Sound H.logic F] : Entailment.Consistent H.logic := by
   apply Entailment.Consistent.of_unprovable (f := ⊥);
   apply not_imp_not.mpr sound.sound;
   exact Kripke.ValidOnFrame.bot_def;
-
-end
-
 
 end Hilbert.Kripke
 
