Foundation/Modal/ModalCompanion/LC.lean
@@ -10,69 +10,72 @@ open Propositional
 open Propositional.Formula (goedelTranslate)
 open Propositional.Formula (atom)
 open Modal
+open Modal.Formula (atom)
 open Modal.Kripke
-
 
 section S4Point3
 
-lemma Hilbert.S4Point3.goedelTranslated_axiomDummett : Hilbert.S4Point3 ⊢! □(□ψᵍ ➝ χᵍ) ➝ □(ψᵍ ➝ χᵍ) := by
+lemma Logic.S4Point3.goedelTranslated_axiomDummett : Logic.S4Point3 ⊢! □(□ψᵍ ➝ χᵍ) ➝ □(ψᵍ ➝ χᵍ) := by
   apply axiomK'!;
   apply nec!;
   apply C!_swap;
   apply deduct'!;
   apply deduct!;
-  have h₁ : [□ψᵍ ➝ χᵍ, ψᵍ] ⊢[Hilbert.S4Point3]! ψᵍ ➝ □ψᵍ := of'! $ Hilbert.goedelTranslated_axiomTc;
-  have h₂ : [□ψᵍ ➝ χᵍ, ψᵍ] ⊢[Hilbert.S4Point3]! ψᵍ := by_axm!;
-  have h₃ : [□ψᵍ ➝ χᵍ, ψᵍ] ⊢[Hilbert.S4Point3]! □ψᵍ ➝ χᵍ := by_axm!;
+  have h₁ : [□ψᵍ ➝ χᵍ, ψᵍ] ⊢[Logic.S4Point3]! ψᵍ ➝ □ψᵍ := of'! $ goedelTranslated_axiomTc;
+  have h₂ : [□ψᵍ ➝ χᵍ, ψᵍ] ⊢[Logic.S4Point3]! ψᵍ := by_axm!;
+  have h₃ : [□ψᵍ ➝ χᵍ, ψᵍ] ⊢[Logic.S4Point3]! □ψᵍ ➝ χᵍ := by_axm!;
   exact h₃ ⨀ (h₁ ⨀ h₂);
 
-private lemma Hilbert.S4Point.lemma₁ : Hilbert.S4 ⊢! □(□φ ➝ □ψ) ➝ □(□φ ➝ ψ) := by
-  apply Hilbert.S4.Kripke.complete.complete;
+@[simp]
+private lemma Logic.S4Point.lemma₁ : Logic.S4 ⊢! □(□φ ➝ □ψ) ➝ □(□φ ➝ ψ) := by
+  apply Logic.S4.Kripke.complete.complete;
   rintro F ⟨_, _⟩ V x h₁ y Rxy h₂;
   apply @h₁ y Rxy h₂;
   apply IsRefl.refl;
 
 namespace Logic
 
-lemma mem_gAxiomPoint3_smallestMC_of_LC : □(□(.atom 0) ➝ (.atom 1)) ⋎ □(□(.atom 1) ➝ (.atom 0)) ∈ Logic.LC.smallestMC := by
-  have : □(□.atom 0 ➝ □.atom 1) ⋎ □(□.atom 1 ➝ □.atom 0) ∈ Logic.LC.smallestMC := by
-    apply Logic.sumNormal.mem₂;
-    use Axioms.Dummett (.atom 0) (.atom 1);
-    simp [Axioms.Dummett, goedelTranslate];
-  apply Propositional.Logic.smallestMC.mdp_S4 ?_ this;
-  apply CAA!_of_C!_of_C!;
-  repeat exact Hilbert.S4Point.lemma₁;
+
+instance : Entailment.HasAxiomPoint3 Logic.LC.smallestMC where
+  Point3 φ ψ := by
+    constructor;
+    apply Modal.Logic.iff_provable.mp;
+    apply Modal.Logic.subst! (L := Logic.LC.smallestMC) (φ := Modal.Axioms.Point3 (.atom 0) (.atom 1)) (s := λ a => match a with | 0 => φ | 1 => ψ | _ => .atom a);
+    have : Logic.LC.smallestMC ⊢! □(□.atom 0 ➝ □.atom 1) ⋎ □(□.atom 1 ➝ □.atom 0) := by
+      apply Logic.sumNormal.mem₂!;
+      use Axioms.Dummett (.atom 0) (.atom 1);
+      simp [Axioms.Dummett, goedelTranslate];
+    apply ?_ ⨀ this;
+    apply CAA!_of_C!_of_C! <;>
+    . apply Entailment.WeakerThan.pbl (𝓢 := Logic.S4)
+      simp;
 
 lemma S4Point3.is_smallestMC_of_LC : Logic.S4Point3 = Logic.LC.smallestMC := by
-  ext φ;
+  apply Logic.iff_equal_provable_equiv.mpr;
+  apply Entailment.Equiv.antisymm_iff.mpr;
   constructor;
-  . intro hφ;
-    induction hφ using Hilbert.Deduction.rec! with
-    | maxm h =>
-      rcases (by simpa using h) with (⟨s, rfl⟩ | ⟨s, rfl⟩ | ⟨s, rfl⟩ | ⟨s, rfl⟩);
-      . apply Logic.sumNormal.mem₁; simp;
-      . apply Logic.sumNormal.mem₁; simp;
-      . apply Logic.sumNormal.mem₁; simp;
-      . exact Logic.sumNormal.subst $ mem_gAxiomPoint3_smallestMC_of_LC;
-    | mdp => apply Logic.sumNormal.mdp <;> assumption;
-    | nec => apply Logic.sumNormal.nec; assumption;
-    | _ => apply Logic.sumNormal.mem₁; simp;
-  . intro hφ;
+  . apply Entailment.weakerThan_iff.mpr;
+    intro φ hφ;
     induction hφ with
-    | mem₁ h => apply Logic.S4Point3.proper_extension_of_S4.subset h;
-    | mdp hφ hψ ihφψ ihψ => apply Modal.Logic.mdp ihφψ ihψ;
-    | subst h ih => apply Modal.Logic.subst ih;
-    | nec h ih => apply Modal.Logic.nec ih;
+    | maxm h => rcases (by simpa using h) with (⟨s, rfl⟩ | ⟨s, rfl⟩ | ⟨s, rfl⟩ | ⟨s, rfl⟩) <;> simp;
+    | mdp ihφψ ihφ => exact ihφψ ⨀ ihφ;
+    | nec ihφ => exact nec! ihφ;
+    | _ => simp;
+  . apply Entailment.weakerThan_iff.mpr;
+    intro _ hφ;
+    induction hφ using Logic.sumNormal.rec! with
+    | mem₁ h => apply WeakerThan.pbl h;
+    | mdp ihφψ ihψ => exact ihφψ ⨀ ihψ;
+    | nec ihφ => exact nec! ihφ;
+    | subst ihφ => apply subst! _ ihφ;
     | mem₂ h =>
       rcases h with ⟨φ, hφ, rfl⟩;
-      apply Hilbert.provable_goedelTranslated_of_provable Hilbert.LC Hilbert.S4Point3 ?_ (by trivial);
+      apply provable_goedelTranslated_of_provable Hilbert.LC Logic.S4Point3 ?_ (by trivial);
       rintro _ ⟨_, ⟨(rfl | rfl), ⟨s, rfl⟩⟩⟩;
-      . apply Logic.S4Point3.proper_extension_of_S4.subset;
-        apply modalCompanion_Int_S4.companion.mp;
-        simp;
-      . suffices Hilbert.S4Point3 ⊢! □(s 0ᵍ ➝ s 1ᵍ) ⋎ □(s 1ᵍ ➝ s 0ᵍ) by simpa [goedelTranslate];
+      . exact WeakerThan.pbl $ modalCompanion_Int_S4.companion.mp (by simp);
+      . suffices Logic.S4Point3 ⊢! □(s 0ᵍ ➝ s 1ᵍ) ⋎ □(s 1ᵍ ➝ s 0ᵍ) by simpa [goedelTranslate];
         apply A!_replace axiomPoint3!;
-        repeat exact Hilbert.S4Point3.goedelTranslated_axiomDummett;
+        repeat exact Logic.S4Point3.goedelTranslated_axiomDummett;
 
 instance modalCompanion_LC_S4Point3 : ModalCompanion Logic.LC Logic.S4Point3 := by
   rw [Logic.S4Point3.is_smallestMC_of_LC];
@@ -90,41 +93,34 @@ end S4Point3
 
 section GrzPoint3
 
-lemma Logic.gGrzPoint3_of_LC : φ ∈ Logic.LC → φᵍ ∈ Logic.GrzPoint3 := by
+lemma Logic.gGrzPoint3_of_LC : φ ∈ Logic.LC → Logic.GrzPoint3 ⊢! φᵍ := by
   intro h;
-  apply GrzPoint3.proper_extension_of_S4Point3.subset;
-  exact modalCompanion_LC_S4Point3.companion.mp h;
+  apply WeakerThan.pbl $ modalCompanion_LC_S4Point3.companion.mp h;
 
 lemma Logic.GrzPoint3.is_largestMC_of_LC : Logic.GrzPoint3 = Logic.LC.largestMC := by
-  ext φ;
+  apply Logic.iff_equal_provable_equiv.mpr;
+  apply Entailment.Equiv.antisymm_iff.mpr;
   constructor;
-  . intro hφ;
-    induction hφ using Hilbert.Deduction.rec! with
+  . apply Entailment.weakerThan_iff.mpr;
+    intro _ hφ;
+    induction hφ with
     | maxm h =>
       rcases (by simpa using h) with (⟨s, rfl⟩ | ⟨s, rfl⟩ | ⟨s, rfl⟩);
-      . apply Logic.sumNormal.mem₁;
-        apply Logic.sumNormal.mem₁;
+      . simp;
+      . simp;
+      . apply WeakerThan.pbl (𝓢 := Logic.LC.smallestMC);
         simp;
-      . apply Logic.sumNormal.subst (φ := □(□((.atom 0) ➝ □(.atom 0)) ➝ (.atom 0)) ➝ (.atom 0)) (s := s);
-        apply Logic.sumNormal.mem₂;
-        simp;
-      . apply Logic.sumNormal.subst (φ := □(□(.atom 0) ➝ (.atom 1)) ⋎ □(□(.atom 1) ➝ (.atom 0))) (s := s);
-        apply Logic.sumNormal.mem₁;
-        rw [←Logic.S4Point3.is_smallestMC_of_LC]
-        simp;
-    | mdp => apply Logic.sumNormal.mdp <;> assumption;
-    | nec => apply Logic.sumNormal.nec; assumption;
-    | _ => apply Logic.sumNormal.mem₁; apply Logic.sumNormal.mem₁; simp;
-  . intro hφ;
-    induction hφ with
-    | mem₁ h =>
-      apply GrzPoint3.proper_extension_of_S4Point3.subset;
-      rwa [Logic.S4Point3.is_smallestMC_of_LC]
-    | mdp hφ hψ ihφψ ihψ => apply Modal.Logic.mdp ihφψ ihψ;
-    | subst h ih => apply Modal.Logic.subst ih;
-    | nec h ih => apply Modal.Logic.nec ih;
-    | mem₂ h =>
-      rcases h with ⟨φ, hφ, rfl⟩; simp;
+    | mdp ihφψ ihφ => exact ihφψ ⨀ ihφ;
+    | nec ihφ => exact nec! ihφ;
+    | _ => simp;
+  . apply Entailment.weakerThan_iff.mpr;
+    intro φ hφ;
+    induction hφ using Logic.sumNormal.rec! with
+    | mem₁ h => apply WeakerThan.pbl $ Logic.S4Point3.is_smallestMC_of_LC ▸ h;
+    | mdp ihφψ ihψ => exact ihφψ ⨀ ihψ;
+    | subst ih => apply subst! _ ih;
+    | nec ih => apply nec! ih;
+    | mem₂ h => rcases h with ⟨φ, hφ, rfl⟩; simp;
 
 instance modalCompanion_LC_GrzPoint3 : ModalCompanion Logic.LC Logic.GrzPoint3 := by
   rw [Logic.GrzPoint3.is_largestMC_of_LC];
@@ -140,7 +136,7 @@ end GrzPoint3
 
 section boxdot
 
-theorem embedding_LC_GLPoint3 {φ : Propositional.Formula ℕ} : φ ∈ Logic.LC ↔ φᵍᵇ ∈ Logic.GLPoint3 := by
+theorem embedding_LC_GLPoint3 {φ : Propositional.Formula ℕ} : φ ∈ Logic.LC ↔ Logic.GLPoint3 ⊢! φᵍᵇ := by
   exact Iff.trans modalCompanion_LC_GrzPoint3.companion Logic.iff_boxdotTranslatedGLPoint3_GrzPoint3.symm
 
 end boxdot
